C-verifier/src/Midend-IVL/Isabelle-UTP/optics/Lens_Algebra.thy
@@ -176,10 +176,10 @@ lemma lens_comp_anhil [simp]: "wb_lens X \<Longrightarrow> 0\<^sub>L ;\<^sub>L X
   by (simp add: zero_lens_def lens_comp_def comp_def)
 
 subsection \<open>Independence laws\<close>
-
+ 
 lemma zero_lens_indep: "0\<^sub>L \<bowtie> X"
   by (auto simp add: zero_lens_def lens_indep_def)
-
+ 
 lemma lens_indep_quasi_irrefl: "\<lbrakk> wb_lens x; eff_lens x \<rbrakk> \<Longrightarrow> \<not> (x \<bowtie> x)"
   by (auto simp add: lens_indep_def ief_lens_def ief_lens_axioms_def, metis (full_types) wb_lens.get_put)
 
